Correctness.v
@@ -1,6 +1,8 @@
 (* Proof of correctness of the translation from core language expression to the Template Coq terms *)
+Require Import Program.Tactics.
 Require Import Ast EvalE Facts CustomTactics String.
 Require Template.WcbvEval.
+Require Import Template.LiftSubst.
 Require Import Template.All.
 
 Require Import List.
@@ -12,7 +14,19 @@ Import Lia.
 Notation "Σ ;;; Γ |- t1 ⇓ t2 " := (WcbvEval.eval Σ Γ t1 t2) (at level 50).
 Notation "T⟦ e ⟧ Σ " := (expr_to_term Σ e) (at level 40).
 
+Tactic Notation "simpl_vars_to_apps" "in" ident(H) :=
+  simpl in H;try rewrite map_app in H; simpl in H;
+  rewrite vars_to_apps_unfold in H;simpl in H.
+
+Tactic Notation "simpl_vars_to_apps" :=
+  simpl;try rewrite map_app; simpl; rewrite vars_to_apps_unfold;simpl.
+
+
 Import InterpreterEnvList.
+
+Lemma expr_closed_term_closed e n Σ:
+  iclosed_n n e = true -> closedn n (T⟦e⟧Σ) = true.
+Admitted.
 
 Lemma map_env_list_size {A B} (f : Ast.name -> A -> B) (ρ : env A) :
   length (map_env_list f ρ) = size ρ.
@@ -82,6 +96,11 @@ Lemma Wcbv_from_value_value v Σ : WcbvEval.value (T⟦ from_val_i v⟧Σ).
 Proof.
 Admitted.
 
+Lemma Wcbv_from_value_closed v Σ n :
+  val_ok v -> closedn n (T⟦ from_val_i v⟧Σ) = true.
+Proof.
+Admitted.
+
 (* This should from the fact that ⇓ is deterministic and
    the fact that value evaluates to itself, but the fact that
    ⇓ is deterministic is not yet proved in Template Coq *)
@@ -90,11 +109,320 @@ Lemma Wcbv_eval_value_determ Σ (Γ:=[]) t1 t2 :
 Proof.
   Admitted.
 
+Lemma type_to_term_closed ty n : closedn n (type_to_term ty) = true.
+Proof.
+Admitted.
+
+(* This should follow from the closedness of  [type_to_term ty] but there is no
+   theorem about substituting to closed terms (yet) in MetaCoq *)
+Lemma type_to_term_subst ty n t : (type_to_term ty) {n:=t} = type_to_term ty.
+Proof.
+Admitted.
+
+Lemma closed_mkApps n t1 t2 :
+  closedn n (mkApps t1 [t2]) = true ->
+  closedn n t1 = true /\ closedn n t2 = true.
+Proof.
+  intros Hc.
+  simpl in Hc. destruct t1;simpl in Hc;
+  try (apply Bool.andb_true_iff in Hc; destruct Hc as [Hct1 HH]);
+  try (apply Bool.andb_true_iff in HH; destruct HH as [Hct2 ?]);split;auto.
+  rewrite forallb_app in HH.
+  apply Bool.andb_true_iff in HH; destruct HH as [Hct2 ?]. simpl in H.
+  apply Bool.andb_true_iff in H; destruct H as [H' ?].
+  simpl. rewrite Hct1. rewrite Hct2. reflexivity.
+  rewrite forallb_app in HH.
+  apply Bool.andb_true_iff in HH; destruct HH as [Hct2 ?]. simpl in H.
+  apply Bool.andb_true_iff in H; destruct H as [H' ?]. assumption.
+Qed.
+
+
+Hint Resolve
+     PeanoNat.Nat.compare_eq
+     Compare_dec.nat_compare_Lt_lt
+     Compare_dec.nat_compare_Gt_gt
+     Compare_dec.leb_correct_conv
+     PeanoNat.Nat.leb_refl : facts.
+Hint Resolve
+     -> PeanoNat.Nat.ltb_lt : facts.
+Hint Resolve
+     -> PeanoNat.Nat.leb_le : facts.
+
+
+Compute ((tRel 1) {0:=tVar "a"}).
+Compute ((tLambda (nNamed"x") (tInd (mkInd "nat" 0) []) (tApp (tRel 1) [tRel 2])) {0:=tRel 0}).
+Compute ( (tApp (tApp (tApp (tApp (tRel 1) [tRel 1]) [tRel 1]) [tRel 1]) [tRel 2]) {0:=tVar "blah"}).
+Compute ( T⟦(eApp (eApp (eApp (eApp (eRel 1) (eRel 1)) (eRel 1)) (eRel 1)) (eRel 2))⟧ []).
+
+Lemma subst_term_subst_env_rec  e :
+  forall v Σ n nm,
+  val_ok v ->
+  iclosed_n (1+n) e = true ->
+  (T⟦e⟧ Σ) {n:=T⟦ from_val_i v ⟧ Σ} =
+  (T⟦subst_env_i_aux n (enEmpty # [nm ~> from_val_i v]) e⟧ Σ).
+Proof.
+  induction e using expr_ind_case;intros v Σ n1 nm nmHv Hc.
+  + (* eRel *)
+    simpl.
+    destruct (Nat.compare n1 n) eqn:Hn.
+    * assert (n1 = n) by auto with facts.
+      subst. simpl in *.
+      assert (Hn0: Nat.leb n n = true) by auto with facts.
+      rewrite Hn0. replace (n - n) with 0 by lia. simpl.
+      assert (closed (T⟦ from_val_i v ⟧ Σ) = true) by (apply Wcbv_from_value_closed;auto).
+      rewrite lift_closed by assumption.
+      reflexivity.
+    * simpl in *.
+      assert (n1 < n) by auto with facts.
+      assert (n < S n1) by auto with facts.
+      exfalso. lia.
+    * simpl in *.
+      assert  (n < S n1) by auto with facts.
+      assert (n1 > n) by auto with facts.
+      assert (Hleb : Nat.leb n1 n = false) by auto with facts.
+      rewrite Hleb. reflexivity.
+  + (* eVar *)
+    reflexivity.
+  + (* eLambda *)
+    simpl in *.
+    rewrite type_to_term_subst.
+    destruct Hc.
+    f_equal. easy.
+  + (* eLetIn *)
+    simpl in *.
+    rewrite type_to_term_subst.
+    apply Bool.andb_true_iff in Hc. destruct Hc as [Hce1 Hce2].
+    f_equal;eauto.
+  + (* eApp *)
+    change ((T⟦ eApp e1 e2 ⟧ Σ)) with ((mkApps (T⟦e1⟧Σ) [T⟦e2⟧Σ])) in *.
+    simpl in Hc.
+    apply Bool.andb_true_iff in Hc. destruct Hc as [Hce1 Hce2].
+    rewrite subst_mkApps.
+    erewrite IHe1 by eauto. simpl.
+    erewrite IHe2 by eauto. reflexivity.
+  + (* eConstr *)
+    simpl. destruct (resolve_constr Σ i n);auto.
+  + (* eConst *)
+    reflexivity.
+  + (* eCase *)
+    simpl in *. destruct p. simpl in *.
+    apply Bool.andb_true_iff in Hc. destruct Hc as [Hce1 Hce2].
+    repeat f_equal.
+    * rewrite type_to_term_subst. reflexivity.
+    * apply IHe; auto.
+    * rewrite_all map_map. simpl.
+      (* we need something similar to [map_ext], but involving [Forall] coming from IH *)
+      apply map_ext.
+      intros a. destruct a.
+      simpl. unfold on_snd. simpl. f_equal.
+Admitted.
+
+
+Lemma subst_term_subst_env e :
+  forall v Σ nm,
+  val_ok v ->
+  iclosed_n 1 e = true ->
+  (T⟦e⟧ Σ) {0:=T⟦ from_val_i v ⟧ Σ} =
+  (T⟦subst_env_i (enEmpty # [nm ~> from_val_i v]) e⟧ Σ).
+Proof.
+  intros.
+  apply subst_term_subst_env_rec;auto.
+Qed.
+
+Lemma subst_env_i_closed_eq :
+  forall (e : expr) (n : nat) (ρ : env expr),
+    iclosed_n 0 e = true ->
+    subst_env_i_aux n ρ e = e.
+Proof.
+  intros e n ρ Hc.
+Admitted.
+
+(* This lemma should be generalized.
+   At least for [subst_env_i_aux n] *)
+Lemma subst_env_compose :
+  forall (nm : Ast.name) (e e1: expr) (ρ : env expr),
+    ForallEnv (fun x => iclosed_n 0 x = true) ρ ->
+    subst_env_i (ρ # [nm ~> e1]) e =
+    subst_env_i (enEmpty # [nm ~> e1])
+                (subst_env_i_aux 1 ρ e).
+Proof.
+  intros nm e e1 ρ.
+  unfold inst_env_i,subst_env_i in *. simpl in *.
+  induction e using expr_ind_case;intros Hfc.
+  + simpl. destruct n.
+    * reflexivity.
+    * simpl. replace (n-0) with n by lia.
+      destruct (lookup_i_norec ρ n) eqn:Hl;auto.
+      simpl. assert (iclosed_n 0 e = true) by
+          (eapply ForallEnv_lookup_i_norec with
+               (P:=fun x : expr => iclosed_n 0 x = true);eauto).
+      symmetry. apply subst_env_i_closed_eq. assumption.
+  + reflexivity.
+  + simpl. f_equal.
+Admitted.
+
+Import Basics.
+Open Scope program_scope.
+
+Lemma ForallEnv_map {A B} (f : A -> B) (ρ : env A) (P : B -> Prop) :
+  ForallEnv (P ∘ f) ρ -> ForallEnv P (map_env f ρ).
+Proof.
+  induction ρ; intros HP; inversion HP; subst; constructor;easy.
+Qed.
+
+Lemma forall_ForallEnv {A} (ρ : env A) (P : A -> Prop) :
+  (forall a : A, P a) -> ForallEnv P ρ.
+Proof.
+  induction ρ;intros HP;constructor;auto.
+Qed.
+
+Lemma ForallEnv_impl:
+  forall (A : Type) (P Q : A -> Prop),
+    (forall a : A, P a -> Q a) -> forall ρ, ForallEnv P ρ -> ForallEnv Q ρ.
+Proof.
+  intros.
+  Admitted.
+
+Lemma eval_expr_i_val_ok  n ρ Σ e v :
+  ForallEnv val_ok ρ ->
+  expr_eval_i n Σ ρ e = Ok v ->
+  val_ok v.
+Admitted.
+
+Lemma from_vConstr_not_lambda :
+  forall (Σ : global_env) (i : Ast.inductive) (n0 : Ast.name) (na : name) (t0 b : term) l,
+    tLambda na t0 b = T⟦ from_val_i (vConstr i n0 l) ⟧ Σ -> False.
+Proof.
+  intros Σ i n0 na t0 b l H.
+  induction l using rev_ind.
+  + simpl in H. destruct (resolve_constr Σ i n0);tryfalse.
+  + simpl_vars_to_apps in H.
+    destruct (T⟦ vars_to_apps (eConstr i n0) (map from_val_i l) ⟧ Σ);tryfalse.
+Qed.
+
+Lemma expr_to_term_not_ind Σ e i u:
+  tInd i u = T⟦e⟧Σ -> False.
+Proof.
+  induction e using expr_ind_case;intros Heq;simpl in Heq;tryfalse.
+  destruct (T⟦ e1 ⟧ Σ);tryfalse.
+  destruct (resolve_constr Σ i0 n);tryfalse.
+  destruct p;tryfalse.
+Qed.
+
+Lemma Wcbv_app_inv Σ Γ e t l :
+  Σ ;;; Γ |- tApp e l ⇓ t ->
+ (exists i n u, Σ ;;; Γ |- e ⇓ tConstruct i n u) \/
+ (exists nm ty b, Σ ;;; Γ |- e ⇓ tLambda nm ty b) \/
+ (exists f n, e = tFix f n) \/
+ (exists i u , Σ ;;; Γ |- e ⇓ tInd i u).
+Proof.
+  intros Happ.
+  inversion Happ;subst; easy.
+Qed.
+
+
+Lemma tFix_eq_inv f l Σ e :
+  tFix f l = T⟦e⟧Σ -> exists fixname var ty1 ty2 b, e = eFix fixname var ty1 ty2 b.
+Proof.
+  destruct e;intros H1;try easy.
+  + simpl in *. now destruct (T⟦ e1 ⟧ Σ).
+  + simpl in *. now destruct (resolve_constr Σ i n).
+  + simpl in *. now destruct p.
+Qed.
+
+Lemma inst_env_eFix_eq_inv (ρ : env val) ty1 ty2 e b fixname var :
+  inst_env_i ρ e = eFix fixname var ty1 ty2 b ->
+  (exists fixname1 var1 ty11 ty21 b1,
+      e = eFix fixname1 var1 ty11 ty21 b1) \/
+  (exists n fixname1 var1 ty11 ty21 b1,
+    e = eRel n /\
+    lookup_i_norec (map_env (fun v => from_val_i v) ρ) n =
+    Some (eFix fixname1 var1 ty11 ty21 b1)).
+Proof.
+  intros H.
+  destruct e;try easy.
+  right.
+  cbn in H.
+  destruct ((lookup_i_norec (map_env (fun v : val => from_val_i v) ρ) (n - 0))) eqn:Hlookup;tryfalse. replace (n-0) with n in * by lia. simpl in *. subst.
+  repeat eexists; easy.
+Qed.
+
+Lemma mkApps_isApp t args :
+  args <> [] -> isApp t = true -> exists args' f, mkApps t args = tApp f (args' ++ args).
+Proof.
+  intros Hneq Happ.
+  destruct args;tryfalse. cbv.
+  cbv in Happ. destruct t;tryfalse. easy.
+Qed.
+
+Lemma mkApps_not_isApp t args :
+  args <> [] -> isApp t = false -> mkApps t args = tApp t args.
+Proof.
+  intros. rewrite <- Bool.not_true_iff_false in *.
+  now apply mkApps_tApp.
+Qed.
+
+
+Lemma mkApps_tApp_exists t args :
+  args <> [] ->
+  exists t' args', mkApps t args = tApp t' args'.
+Proof.
+  intros Hneq.
+  destruct (isApp t) eqn:Happ.
+  * specialize (mkApps_isApp _ _ Hneq Happ) as H;firstorder.
+  * specialize (mkApps_not_isApp _ _ Hneq Happ) as H;firstorder.
+Qed.
+
+Ltac destruct_one_ex_named :=
+  let tac x H := let x_new := fresh x in (destruct H as [x_new H]) in
+    match goal with
+      | [H : (exists x1, _) |- _] => tac x1 H
+    end.
+
+Ltac destruct_one_ex_named' Hex :=
+  let tac x H := (destruct H as [x H]) in
+  match Hex with
+  | ex (fun x => _) => tac x Hex
+  end.
+
+
+Ltac destruct_ex_named := repeat (destruct_one_ex_named).
+
+(* Since [mkApps] a smart constructor, it should be semantically equivalent to ordinary [tApp] *)
+Lemma mkApps_sound Σ Γ e l t :
+  Σ ;;; Γ |- mkApps e l ⇓ t ->
+  Σ ;;; Γ |- tApp e l ⇓ t.
+Proof.
+  Admitted.
+
+Compute (T⟦vars_to_apps (eRel 0) [eRel 1; eRel 2;eRel 3;eRel 4]⟧nil).
+Lemma expr_to_term_apps f a args Σ :
+  T⟦vars_to_apps f (args ++ [a])⟧Σ = tApp (T⟦f⟧Σ) (map (fun e => T⟦e⟧Σ) (args++[a])).
+Proof.
+  induction args using rev_ind.
+  + simpl. destruct (T⟦ f ⟧ Σ);auto.
+  (* rewrite vars_to_apps_unfold. simpl. *)
+  (* rewrite IHargs. f_equal. rewrite map_app. *)
+  (* reflexivity. intros H1.  apply H. *)
+Admitted.
+
+
+(* Lemma tConstr_inv i1 i2 nm1 nm2 u Σ l : *)
+(*   tConstruct i1 nm1 u = T⟦ from_val_i (vConstr i2 nm2 l) ⟧ Σ -> *)
+(*   i1 = i2 /\ nm1 = nm2 /\ l = []. *)
+(* Proof. *)
+(*   induction l using rev_ind. *)
+(*   simpl. destruct (resolve_constr Σ i2 nm2);tryfalse. *)
+(*   Focus 2. *)
+(*                simpl_vars_to_apps in IH. *)
+(*            inversion IH;subst. *)
 
 Theorem expr_to_term_sound n ρ Σ1 Σ2 (Γ:=[]) (e1 e2 : expr) (t : term) (v : val) :
-  inst_env_i ρ e1 = e2 ->
+  env_ok ρ ->
   Σ2 ;;; Γ |- T⟦e2⟧Σ1 ⇓ t ->
   expr_eval_i n Σ1 ρ e1 = Ok v ->
+  inst_env_i ρ e1 = e2 ->
+  iclosed_n 0 e2 = true ->
   t = T⟦from_val_i v⟧Σ1.
 Proof.
   revert dependent v.
@@ -104,12 +432,11 @@ Proof.
   revert dependent e1.
   induction n.
   - intros;tryfalse.
-  - intros e1 e2 ρ t v Henv HT He.
+  - intros e1 e2 ρ t v Hρ_ok HT He Henv Hc.
     destruct e1.
     + (* eRel*)
       autounfold with facts in *. simpl in *.
       destruct (lookup_i ρ n0) eqn:Hlookup;tryfalse. simpl in He;inversion He;subst.
-
       assert (Hn0 : n0 < size ρ \/ size ρ <= n0) by lia.
       destruct Hn0 as [Hlt | Hge].
       * destruct (inst_env_i_in _ _ Hlt) as [v1 HH].
@@ -129,8 +456,70 @@ Proof.
       reflexivity.
     + (* eLetIn *)
       autounfold with facts in *. simpl in HT. simpl in He.
-      destruct (expr_eval_general n false Σ1 ρ e1_1);tryfalse.
+      destruct (expr_eval_general n false Σ1 ρ e1_1) eqn:He1;tryfalse.
       rewrite <- Henv in HT.
       unfold inst_env_i,subst_env_i in Henv. simpl in Henv.
-      simpl in *. inversion HT. subst.
+      simpl in *. inversion_clear HT.
+      rewrite <- Henv in Hc.
+      simpl in Hc.
+      apply Bool.andb_true_iff in Hc. destruct Hc as [Hce1 Hce2].
+      specialize (IHn _ _ _ _ _ Hρ_ok H He1 eq_refl Hce1) as IH.
+      rewrite IH in H0.
+      assert (Hv0_ok : val_ok v0) by (eapply eval_expr_i_val_ok;eauto).
+      (* An important bit of the proof is to show how substitution of the environment into an expression
+         interacts with the substitution of MetaCoq *)
+      rewrite subst_term_subst_env with (nm:=n0) in H0 by auto.
+
+      assert (Hρ_ok1 : ForallEnv val_ok (ρ # [n0 ~> v0])).
+      { constructor. eapply eval_expr_i_val_ok;eauto. assumption. }
+      eapply IHn;eauto. apply subst_env_compose.
+      apply ForallEnv_map.
+      eapply ForallEnv_impl with (fun v => val_ok v).
+      { intros; apply from_value_closed;assumption. }
+      assumption.
+      apply subst_env_iclosed. simpl. assumption.
+      constructor. apply from_value_closed;assumption.
+      constructor.
+    + (* eApp *)
+      autounfold with facts in *. simpl in He.
+      pose proof HT as HT1.
+      rewrite <- Henv in HT.
+      destruct (expr_eval_general n false Σ1 ρ e1_1) eqn:He1;tryfalse.
+      2 :
+        { try (destruct (expr_eval_general n false Σ1 ρ e1_2) eqn:He2);tryfalse. }
+      change (T⟦inst_env_i ρ (eApp e1_1 e1_2)⟧Σ1) with
+             (mkApps (T⟦inst_env_i ρ  e1_1⟧Σ1) [T⟦inst_env_i ρ e1_2⟧Σ1]) in HT.
+      specialize (mkApps_sound _ _ _ _ _ HT) as HT'. clear HT.
+      rewrite <- Henv in Hc.
+      simpl in Hc.
+      apply Bool.andb_true_iff in Hc. destruct Hc as [Hce1 Hce2].
+      assert (Hneq : [T⟦ inst_env_i ρ e1_2 ⟧ Σ1] <> []) by easy.
+      destruct_ex_named.
+      (* apply Wcbv_app_inv in HT'. *)
+      destruct v0;destruct (expr_eval_general n false Σ1 ρ e1_2) eqn:He2;tryfalse.
+      * (* application evaluates to a construtor *)
+        inversion_clear He.
+        inversion HT';subst.
+        ** exfalso. now eapply from_vConstr_not_lambda.
+        ** specialize (tFix_eq_inv _ _ _ _ H) as HH.
+           destruct_ex_named. rewrite HH in H. simpl in H.
+           inversion H. subst. cbn in H1. inversion H1. subst. clear H1. clear H.
+           rewrite type_to_term_subst in H5.
+           apply inst_env_eFix_eq_inv in HH.
+           destruct HH.
+           *** destruct_ex_named. subst. destruct n;tryfalse.
+           *** destruct_ex_named. destruct H.
+               subst. destruct n;tryfalse. simpl in He1.
+               (* relate [lookup_i_norec] and [lookup_i] *)
+               admit.
+        ** exfalso; now eapply expr_to_term_not_ind.
+        ** specialize (IHn _ _ _ _ _ Hρ_ok H2 He1 eq_refl Hce1) as IH.
+           simpl in IH.
+           inversion H4;subst. inversion H6;subst. inversion H4;subst.
+           assert (l = []). admit. (* from inversion of IH *)
+           subst.
+           assert (H : y = T⟦ from_val_i v0 ⟧ Σ1) by easy.
+           subst.
+           rewrite IH. simpl.
+           destruct (resolve_constr Σ1 i n0); reflexivity.
 Admitted.
